more int approx

src/examples/Kuiper.IntApprox.fst
@@ -1,8 +1,11 @@
 module Kuiper.IntApprox
 
+#lang-pulse
+
 open Kuiper
 open Kuiper.Approximates
 open Kuiper.Approximates.U32
+open Kuiper.Seq.Common
 module U32 = FStar.UInt32
 
 (* To expose the definitions of to_real and v_approximates. *)
@@ -21,3 +24,82 @@ let lem' (z x y : u32)
   : Lemma (requires z %~ (to_real x +. to_real y))
           (ensures  FStar.UInt32.(z == x +%^ y))
   = ()
+
+(* Strenghten the spec of a reduction *)
+
+fn reduce (#et:Type0) {| scalar et, real_like et |}
+  (len:nat) (a : larray u32 len) (#s : seq u32)
+  (#r : erased (seq real))
+  preserves a |-> s ** pure (s %~ r)
+  returns   res : u32
+  ensures   pure (res %~ seq_fold_left (+.) 0.0R r)
+{
+  admit(); // Intentional, to not importa HReduce here.
+}
+
+let get_int_from_real_approx (x:u32) (r:real)
+  : Ghost (erased int)
+          (requires x %~ r)
+          (ensures  fun i -> r == Real.of_int i /\ UInt32.v x == i % pow2 32)
+  = FStar.IndefiniteDescription.indefinite_description_ghost int
+      (fun i -> r == Real.of_int i /\ UInt32.v x == i % pow2 32)
+
+#push-options "--z3rlimit 30"
+let rec lem_seq_approx (s : seq u32) (i : int)
+  : Lemma (requires Real.of_int i == seq_fold_left (+.) 0.0R (seq_map to_real s))
+          (ensures  i % (pow2 32) == U32.v (seq_fold_left add zero s))
+          (decreases Seq.length s)
+  = match view_seq s with
+    | SNil -> ()
+    | SCons hd tl ->
+      let i' = i - U32.v hd in
+      lemma_seq_fold_left_sum 0.0R (+.) seq![to_real hd] (seq_map to_real tl);
+      assert (s == seq![hd] `Seq.append` tl);
+      assert (Seq.equal (seq_map to_real s)
+                         (seq![to_real hd] `Seq.append` seq_map to_real tl));
+      assert (Seq.equal (seq_map to_real seq![hd])
+                         seq![to_real hd]);
+      assert (seq_fold_left (+.) 0.0R seq![to_real hd] 
+              == to_real hd);
+      assert (seq_fold_left (+.) 0.0R (seq_map to_real s)
+               == to_real hd +. seq_fold_left (+.) 0.0R (seq_map to_real tl));
+      lem_seq_approx tl (i - U32.v hd);
+      calc (==) {
+        i % pow2 32;
+        == {}
+        (i' + U32.v hd) % pow2 32;
+        == { Math.Lemmas.modulo_distributivity i' (U32.v hd) (pow2 32) }
+        (i' % pow2 32 + U32.v hd % pow2 32) % pow2 32;
+        == {}
+        (U32.v (seq_fold_left add zero tl) % pow2 32 + U32.v hd % pow2 32) % pow2 32;
+        == {}
+        (U32.v hd % pow2 32 + U32.v (seq_fold_left add zero tl) % pow2 32) % pow2 32;
+        == { Math.Lemmas.modulo_distributivity
+                 (U32.v hd) (U32.v (seq_fold_left add zero tl)) (pow2 32) }
+        (U32.v hd + U32.v (seq_fold_left add zero tl)) % pow2 32;
+        == {}
+        U32.v (hd `add` seq_fold_left add zero tl);
+        == { lemma_seq_fold_left_sum #u32 zero add seq![hd] tl }
+        U32.v (seq_fold_left add zero s);
+        == { Math.Lemmas.small_mod (U32.v (seq_fold_left add zero s)) (pow2 32) }
+        U32.v (seq_fold_left add zero s) % pow2 32;
+      };
+      ()
+#pop-options
+
+(* A stronger exact spec for reduce on u32s, proven from the approximate spec. *)
+fn reduce_u32 (len:nat) (a : larray u32 len) (#s : seq u32)
+  preserves a |-> s 
+  returns   res : u32
+  ensures   pure (U32.v res == seq_fold_left add zero s)
+{
+  let res = reduce #u32 len a #s #(seq_map to_real s);
+  ();
+  let rr = seq_fold_left (+.) 0.0R (seq_map to_real s);
+  assert pure (res %~ rr);
+  assert pure (exists (i:int). rr == Real.of_int i /\ i % pow2 32 == U32.v res);
+  let i = get_int_from_real_approx res rr;
+  lem_seq_approx s i;
+  assert pure (res %~ rr);
+  res
+}
